lib/Apply_Debug_Test.thy
@@ -10,9 +10,141 @@
  *)
 
 theory Apply_Debug_Test
-imports Apply_Debug Apply_Trace_Cmd
+imports Apply_Debug
 begin
 
+chapter \<open>Apply_Debug\<close>
 
-end
+text \<open>
+ Apply_debug can be invoked as a backwards refinement step (wherever "apply" works). It invokes
+ the given proof method (expression) in a managed thread and blocks when it encounters a special
+ "#break" method. Either this is written as part of the definition in an inner method written in Eisbach,
+ or appears directly in the invoked method.
+ Once a break point is hit, the proof thread blocks and the command returns with whatever the proof
+ state was at the breakpoint.
+
+ The provided "continue" command allows for execution to resume. Note that regular proof commands
+ can be written between continue commands and method execution will continue as if that were
+ the proof state at the break point. This can allow for debugging methods without necessarily rewriting
+ their implementation.
+
+ Some interactive markup is given in jEdit, including showing in real-time the currently executing
+ method. When printing a proof state (via apply_debug or continue) the associated breakpoint
+ will be highlighted (or the final invoked method
+ if the proof thread has finished). Note that this includes marking up an Eisbach definition.
+
+ Finally the "finish" command will resume execution and ignore all further breakpoints.
+
+ Outside of an apply_debug invocation the #break method is ignored.
+\<close>
+
+method some_break = #break
+
+lemma assumes B: B
+  shows "A \<Longrightarrow> A \<and> B \<and> A \<and> A"
+  apply (rule conjI, #break, assumption) (* #break is ignored here *)
+  apply_debug (rule conjI, #break, some_break, #break, assumption?)+
+  continue
+  continue
+    apply (rule B)
+  continue
+  finish
+  apply assumption
+  done
+
+section \<open>Tags\<close>
+
+text \<open>
+  Tags can be used to filter the kind of breakpoints that are hit by any given breakpoint
+  invocation. By default apply_debug will only hit untagged breakpoints, if any tags are given
+  then both untagged breakpoints and those matching the given tags will trigger a break.
+  Each breakpoint can be given 0 or 1 tags.
+
+  For more fine-grained control, each "continue" may also be given a list of tags. This expands
+  the list of breakpoint tags that can be hit only for the duration of that particular continue.
+\<close>
+
+method my_conjI = (#break "conjI", rule conjI)
+method my_assumption = (#break "assumption", assumption)
+
+lemma "A \<Longrightarrow> A \<and> A \<and> A \<and> A"
+  apply_debug (my_conjI, my_assumption) (* no breakpoints hit *)
+
+  apply_debug (tags "assumption")
+    (#break, my_conjI, my_assumption)
+    continue
+    continue
+
+  apply_debug (tags "conjI")
+    (my_conjI, my_assumption)
+  continue (tags "assumption")
+  finish
+
+
+  continue
+  finish
+  apply_debug (tags "assumption", "conjI")
+    (my_conjI, my_assumption)
+  continue
+  finish
+  continue
+  finish
+  by assumption
+
+
+named_theorems rule3
+
+method bazz for C :: int uses rule1 rule2 declares rule3 =
+  (match premises in H[OF rule2]:"PROP G" for G \<Rightarrow> \<open>#break\<close>)
+
+
+
+schematic_goal Z:
+  assumes AC: "A \<Longrightarrow> C"
+  assumes BA: "B \<Longrightarrow> A"
+  assumes AB: "A \<Longrightarrow> B"
+  assumes A: "A"
+  assumes rule1: "ZZZ"
+  assumes A: "A"
+  assumes C
+  shows "(A \<Longrightarrow> ?C) \<Longrightarrow> D \<Longrightarrow> A \<and> B \<and> C"
+
+  apply (intro conjI)
+  prefer 2
+
+  apply_debug (match premises in H:"PROP C" for C \<Rightarrow>
+        \<open>#break, bazz 4 rule1: AB rule2: A\<close>)
+    term ?C (* C from match is bound *)
+    continue
+    term ?C (* C is now argument to bazz *)
+    term ?G (* G is bound from inner match from bazz *)
+    thm rule1 (* bound to AB from call site *)
+    thm rule2 (* bound to A from call site *)
+    thm H (* bound to match result from bazz (shadows outermost result) *)
+    finish
+ oops
+
+lemma
+  assumes AB: "A \<Longrightarrow> B"
+  assumes BA: "B \<Longrightarrow> A"
+  assumes BC: "B \<Longrightarrow> C"
+  assumes CB: "C \<Longrightarrow> B"
+  assumes CD: "C \<Longrightarrow> D"
+  assumes DC: "D \<Longrightarrow> C"
+  assumes DE: "D \<Longrightarrow> E"
+  assumes ED: "E \<Longrightarrow> D"
+  assumes FE: "F \<Longrightarrow> E"
+  assumes EF: "E \<Longrightarrow> F"
+  assumes E: "E"
+  shows
+  "A"
+
+  apply_debug ((((#break, rule assms, #break, rule assms,#break, rule assms, #break, rule assms, #break,
+                rule assms, #break, rule assms, #break, rule assms)));fail)
+
+  continue 3
+  continue 11
+  continue
+done
+
 end
